hoare_repeat without proof

swotarfe_andufotions/src/Hoare.v
@@ -632,3 +632,216 @@ Proof.
     + trivial.
     + apply Hb with st; try split; assumption.
 Qed.
+
+Module RepeatExercise.
+
+Inductive com :=
+  | CSkip   : com
+  | CAss    : id   -> aexp -> com
+  | CSeq    : com  -> com  -> com
+  | CIf     : bexp -> com  -> com  -> com
+  | CWhile  : bexp -> com  -> com
+  | CRepeat : com  -> bexp -> com.
+
+(* Exercise: 4 stars (hoare_repeat) *)
+
+Notation "'SKIP'" :=
+  CSkip.
+Notation "x '::=' a" :=
+  (CAss x a) (at level 60).
+Notation "c1 ;; c2" :=
+  (CSeq c1 c2) (at level 80, right associativity).
+Notation "'WHILE' b 'DO' c 'END'" :=
+  (CWhile b c) (at level 80, right associativity).
+Notation "'IFB' c1 'THEN' c2 'ELSE' c3 'FI'" :=
+  (CIf c1 c2 c3) (at level 80, right associativity).
+Notation "'REPEAT' c 'UNTIL' b 'END'" :=
+  (CRepeat c b) (at level 80, right associativity).
+
+Reserved Notation "c1 '/' st '⇓' st'" (at level 40, st at level 39).
+
+Inductive ceval : com -> state -> state -> Prop :=
+  | E_Skip : forall st, SKIP / st ⇓ st
+  | E_Ass  : forall st x ae,  (x ::= ae) / st ⇓ (update st x (aeval st ae))
+  | E_Seq  : forall st st' st'' c1 c2,
+               c1 / st  ⇓ st'  ->
+               c2 / st' ⇓ st'' ->
+               (c1 ;; c2) / st ⇓ st''
+  | E_IfTrue  : forall st st' ct ce be,
+               beval st be = true ->
+               ct / st ⇓ st'   ->
+               (IFB be THEN ct ELSE ce FI) / st ⇓ st'
+  | E_IfFalse : forall st st' ct ce be,
+               beval st be = false ->
+               ce / st ⇓ st'    ->
+               (IFB be THEN ct ELSE ce FI) / st ⇓ st'
+  | E_WhileEnd : forall st c be,
+               beval st be = false ->
+               (WHILE be DO c END) / st ⇓ st
+  | E_WhileLoop : forall st st' st'' c be,
+               beval st be = true ->
+               c / st ⇓ st' ->
+               (WHILE be DO c END) / st' ⇓ st'' ->
+               (WHILE be DO c END) / st  ⇓ st''
+  | E_RepeatEnd : forall st st' c be,
+               c / st ⇓ st' ->
+               beval st' be = true ->
+               (REPEAT c UNTIL be END) / st ⇓ st'
+  | E_RepeatLoop : forall st st' st'' c be,
+               c / st ⇓ st' ->
+               beval st' be = false ->
+               (REPEAT c UNTIL be END) / st' ⇓ st'' ->
+               (REPEAT c UNTIL be END) / st ⇓ st''
+   where "c1 '/' st '⇓' st'" := (ceval c1 st st').
+
+Definition hoare_triple
+        (P : Assertion) (c : com) (Q : Assertion) : Prop :=
+        forall st st',
+        c / st ⇓ st' ->
+        P st ->
+        Q st'.
+
+Notation "{{ P }} c {{ Q }}" := (hoare_triple P c Q) (at level 90,
+        c at next level) : hoare_spec_scope.
+
+Definition ex1_repeat :=
+  REPEAT
+    X ::= ANum 1;;
+    Y ::= APlus (AId Y) (ANum 1)
+UNTIL (BEq (AId X) (ANum 1)) END.
+
+Theorem ex1_repeat_works :
+  ex1_repeat / empty_state ⇓
+               update (update empty_state X 1) Y 1.
+Proof.
+  eapply E_RepeatEnd.
+  eapply E_Seq.
+  apply E_Ass.
+  apply E_Ass.
+  reflexivity.
+Qed.
+
+Theorem hoare_repeat_weak : forall Q b c,
+  {{ Q }} c {{ Q }} ->
+  {{ Q }} REPEAT c UNTIL b END {{ fun st => Q st /\ bassn b st }}.
+Proof.
+  intros Q b c Hfl st st' Hc Hp.
+  remember (REPEAT c UNTIL b END) as rcom.
+  induction Hc; inversion Heqrcom; subst.
+    + apply bexp_eval_true  in H. split.
+      - apply Hfl with st; assumption.
+      - assumption.
+    + apply bexp_eval_false in H.
+      apply IHHc2. trivial.
+      apply Hfl with st; try split; assumption.
+Qed.
+
+Theorem hoare_repeat : forall P Q b c,
+  {{ P }} c {{ Q }} ->
+  {{ fun st => Q st /\ ~ bassn b st }} c {{ Q }} ->
+  {{ P }} REPEAT c UNTIL b END {{ fun st => Q st /\ bassn b st }}.
+Proof. Admitted.
+
+(* OLD RULES *)
+
+Theorem hoare_consequence_pre : forall (P P' Q : Assertion) c,
+  {{ P' }} c {{ Q }} ->
+  P ->> P' ->
+  {{ P  }} c {{ Q }}.
+Proof.
+  intros.
+  intros st st' Hc Hp.
+  unfold hoare_triple in H.
+  apply H with st.
+  - assumption.
+  - apply H0. assumption.
+Qed.
+
+Theorem hoare_seq : forall P Q R c1 c2,
+  {{ Q }} c2 {{ R }} ->
+  {{ P }} c1 {{ Q }} ->
+  {{ P }} c1 ;; c2 {{ R }}.
+Proof.
+  intros P Q R c1 c2 Hc2 Hc1.
+  intros st st' HSeq Hp.
+  inversion HSeq; subst.
+  apply Hc1 in H1. apply H1 in Hp.
+  apply Hc2 in H4. apply H4 in Hp.
+  assumption.
+Qed.
+
+Theorem hoare_consequence_post : forall (P Q Q' : Assertion) c,
+  {{ P }} c {{ Q' }} ->
+  Q' ->> Q ->
+  {{ P }} c {{ Q  }}.
+Proof.
+  intros.
+  intros st st' Hc Hp.
+  apply H0.
+  apply H with st; assumption.
+Qed.
+
+Definition assn_sub X a P : Assertion :=
+  fun (st : state) =>
+    P (update st X (aeval st a)).
+
+Notation "P [ X |-> a ]" := (assn_sub X a P) (at level 10).
+
+Theorem hoare_asgn : forall Q X a,
+  {{ Q [X |-> a] }} (X ::= a) {{ Q }}.
+Proof.
+  unfold assn_sub.
+  unfold hoare_triple.
+  intros Q X a st st' Hc Hp.
+  inversion Hc; subst.
+  assumption.
+Qed.
+
+(* / OLD RULES *)
+
+Theorem hoare_repeat_ex1 :
+  {{ fun st => st X > 0 }}
+    REPEAT
+      Y ::= AId X ;;
+      X ::= AMinus (AId X) (ANum 1)
+    UNTIL (BEq (AId X) (ANum 0)) END
+  {{ fun st => st X = 0 /\ st Y > 0 }}.
+Proof.
+  apply hoare_consequence_post with
+    ((fun st : state => st Y > 0 /\ bassn (BEq (AId X) (ANum 0)) st)).
+  - apply hoare_repeat.
+    + eapply hoare_seq.
+      * apply hoare_asgn.
+      * eapply hoare_consequence_pre.
+        { apply hoare_asgn. }
+        { unfold assn_sub. intros st H.
+          simpl. rewrite update_neq.
+          { rewrite update_eq. assumption. }
+          { intros contra; inversion contra. }
+        }
+    + eapply hoare_seq.
+      * apply hoare_asgn.
+      * eapply hoare_consequence_pre.
+        { apply hoare_asgn. }
+        { unfold assn_sub. intros st H.
+          simpl. rewrite update_neq.
+          { rewrite update_eq. destruct H.
+            unfold bassn in H0. simpl in H0.
+            unfold not in H0.
+            destruct (st X).
+            - apply ex_falso_quodlibet. apply H0. reflexivity.
+            - omega.
+          }
+          intros contra; inversion contra.
+        }
+  - unfold bassn. simpl. intros st H.
+    destruct H.
+    split; try assumption.
+    destruct (st X).
+    + trivial.
+    + inversion H0.
+Qed.
+
+(* END hoare_repeat. *)
+
+End RepeatExercise.
